src/named/Rule.v
@@ -115,7 +115,7 @@ Lemma invert_eq_term_eq_rule_term_eq_rule c c' e1 e2 e1' e2' t t'
 Proof. solve_invert_constr_eq_lemma. Qed.
 Hint Rewrite invert_eq_term_eq_rule_term_eq_rule : term.
 
-Notation well_scoped := (well_scoped (V:=V) (A:=term) (Substable0:=@substable_term V V_Eqb)).
+Notation well_scoped := (well_scoped (V:=V) (A:=term)).
   
 Definition ws_rule r : Prop :=
   match r with
